hol-light/stateful/holSemanticsExtraScript.sml
@@ -5,6 +5,10 @@ val _ = new_theory"holSemanticsExtra"
 
 val mem = ``mem:'U->'U->bool``
 
+val is_std_interpretation_is_type = store_thm("is_std_interpretation_is_type",
+  ``is_std_interpretation i ⇒ is_std_type_assignment (FST i)``,
+  Cases_on`i` >> simp[is_std_interpretation_def])
+
 val typesem_inhabited = store_thm("typesem_inhabited",
   ``is_set_theory ^mem ⇒
     ∀tyenv τ δ ty.
@@ -30,85 +34,115 @@ val typesem_Fun = store_thm("typesem_Fun",
     Funspace (typesem τ δ dom) (typesem τ δ rng)``,
   rw[is_std_type_assignment_def,typesem_def])
 
+val termsem_clauses = store_thm("termsem_clauses",
+  ``(∀v i x ty. termsem v i (Var x ty) = (SND v) (x,ty)) ∧
+    (∀v i name ty. termsem v i (Const name ty) = (SND i) name ty (FST v)) ∧
+    (∀v i t1 t2. termsem v i (Comb t1 t2) = termsem v i t1 ' (termsem v i t2)) ∧
+    (∀v i x ty b. termsem v i (Abs x ty b) =
+      Abstract (typesem (FST v) (FST i) ty) (typesem (FST v) (FST i) (typeof b))
+        (λm. termsem (FST v, ((x,ty) =+ m) (SND v)) i b))``,
+  rpt conj_tac >> Cases >> Cases >> rw[termsem_def])
+
+val termsem_niceind = store_thm("termsem_niceind",
+  ``∀P.
+    ((∀v i x ty. P v i (Var x ty)) ∧
+     (∀v i name ty. P v i (Const name ty)) ∧
+     (∀v i t1 t2. P v i t1 ∧ P v i t2 ⇒ P v i (Comb t1 t2)) ∧
+     (∀v i x ty b. (∀m. P (FST v, ((x,ty) =+ m) (SND v)) i b) ⇒
+                   P v i (Abs x ty b)))
+    ⇒ ∀v i t. P (v:'U valuation) (i:'U interpretation) t``,
+  rw[] >>
+  Q.ISPEC_THEN`λ(^mem) (v1,v2) i t. P (v1,v2) i t`mp_tac termsem_ind >>
+  Cases_on`v`>> simp[])
+
 val termsem_typesem = store_thm("termsem_typesem",
   ``is_set_theory ^mem ⇒
-    ∀sig τ σ i tm.
-      is_type_valuation τ ∧
-      is_type_assignment (FST sig) (FST i) ∧
-      is_term_valuation τ (FST i) σ ∧
-      is_term_assignment (SND sig) (FST i) (SND i) ∧
+    ∀sig v i tm.
+      is_valuation (FST i) v ∧
+      is_interpretation sig i ∧
       is_std_type_assignment (FST i) ∧
       term_ok sig tm
       ⇒
-      termsem τ σ i tm <: typesem τ (FST i) (typeof tm)``,
-  simp[PULL_FORALL] >> gen_tac >> Q.ID_SPEC_TAC`mem` >>
-  ho_match_mp_tac termsem_ind >> Cases_on`sig` >>
+      termsem v i tm <: typesem (FST v) (FST i) (typeof tm)``,
+  strip_tac >> gen_tac >>
+  ho_match_mp_tac termsem_niceind >> Cases_on`sig` >>
   strip_tac >- (
-    simp[termsem_def,is_term_valuation_def,term_ok_def] >>
+    Cases >> Cases >>
+    simp[termsem_clauses,is_valuation_def,is_term_valuation_def
+        ,is_interpretation_def,term_ok_def] >>
     rw[] >> metis_tac[typesem_inhabited] ) >>
   strip_tac >- (
-    simp[termsem_def,is_term_assignment_def,FEVERY_ALL_FLOOKUP,term_ok_def] >>
+    Cases >> Cases >>
+    simp[termsem_clauses,is_valuation_def,is_interpretation_def
+        ,is_term_assignment_def,FEVERY_ALL_FLOOKUP,term_ok_def] >>
     metis_tac[] ) >>
   strip_tac >- (
-    simp[termsem_def,term_ok_def] >>
+    Cases >>
+    simp[termsem_clauses,term_ok_def] >>
     rw[] >> imp_res_tac typesem_Fun >> fs[] >>
     match_mp_tac (UNDISCH apply_in_rng) >>
     HINT_EXISTS_TAC >> simp[] ) >>
-  simp[termsem_def,term_ok_def] >>
+  Cases >> Cases >>
+  simp[termsem_clauses,term_ok_def] >>
   rw[] >> imp_res_tac typesem_Fun >> rw[] >>
   match_mp_tac (UNDISCH abstract_in_funspace) >>
   fs[] >> rw[] >>
   first_x_assum match_mp_tac >>
-  fs[is_term_valuation_def] >>
+  fs[is_valuation_def,is_term_valuation_def] >>
   simp[combinTheory.APPLY_UPDATE_THM] >>
   rw[] >> rw[])
 
 val Equalsem =
   is_std_interpretation_def
   |> SPEC_VAR |> snd
-  |> Q.SPECL [`FST (i:'U interp)`,`SND i`]
+  |> Q.SPECL [`FST (i:'U interpretation)`,`SND i`]
   |> concl |> rhs
   |> strip_conj |> tl |> hd
   |> strip_forall |> snd |> rhs
-  |> dest_abs |> snd
+  |> C (curry mk_comb) ``FST(v:'U valuation)``
+  |> beta_conv
 
 val termsem_Equal = store_thm("termsem_Equal",
-  ``∀τ σ i ty.
+  ``∀v i ty.
       is_std_interpretation i ⇒
-      termsem τ σ i (Equal ty) = ^Equalsem``,
-  Cases_on`i` >>
-  rw[is_std_interpretation_def,termsem_def])
+      termsem v i (Equal ty) = ^Equalsem``,
+  Cases >> Cases >>
+  rw[is_std_interpretation_def,termsem_clauses])
 
-(*
-val tac =
+val term_ok_equation = store_thm("term_ok_equation",
+  ``is_std_sig sig ⇒
+      (term_ok sig (s === t) ⇔
+        term_ok sig s ∧ term_ok sig t ∧
+        welltyped t ∧ welltyped s ∧
+        typeof t = typeof s ∧
+        type_ok (FST sig) (typeof s))``,
+  Cases_on`sig` >> rw[equation_def,term_ok_def,type_ok_def,is_std_sig_def] >>
+  rw[EQ_IMP_THM] >>
+  qexists_tac`[(typeof s,Tyvar "A")]` >>
+  rw[holSyntaxLibTheory.REV_ASSOCD_def])
+
+val termsem_equation = store_thm("termsem_equation",
+  ``is_set_theory ^mem ⇒
+    ∀sig v i s t.
+    is_structure sig v i ∧
+    term_ok sig (s === t)
+    ⇒ termsem v i (s === t) = Boolean (termsem v i s = termsem v i t)``,
+  rw[is_structure_def] >> rfs[term_ok_equation] >>
+  simp[equation_def,termsem_clauses,termsem_Equal] >>
+  imp_res_tac is_std_interpretation_is_type >>
   qho_match_abbrev_tac`Abstract a b f ' x ' y = z` >>
   `Abstract a b f ' x = f x` by (
     match_mp_tac (UNDISCH apply_abstract) >>
     unabbrev_all_tac >> simp[] >>
-    TRY (conj_tac >-
-    termsem_typesem
-    metis_tac[semantics_typeset,semantics_11]) >>
-    match_mp_tac ABSTRACT_IN_FUNSPACE >>
-    metis_tac[semantics_typeset,WELLTYPED,boolean_in_boolset] ) >>
+    TRY (conj_tac >- metis_tac[termsem_typesem]) >>
+    match_mp_tac (UNDISCH abstract_in_funspace) >>
+    simp[boolean_in_boolset] ) >>
   simp[Abbr`f`,Abbr`b`] >>
   qho_match_abbrev_tac`Abstract a b f ' y = z` >>
   `Abstract a b f ' y = f y `  by (
     match_mp_tac (UNDISCH apply_abstract) >>
     unabbrev_all_tac >> simp[] >>
-    metis_tac[semantics_typeset,semantics_11,boolean_in_boolset] ) >>
-  unabbrev_all_tac >> simp[]
-
-val termsem_equation = store_thm("termsem_equation",
-  ``is_set_theory ^mem ⇒
-    ∀sig τ σ i s t mst.
-    is_type_valuation τ ∧
-    is_term_valuation τ (FST i) σ ∧
-    is_interpretation sig i ∧
-    typeof s = typeof t ∧
-    mst = Boolean (termsem τ σ i s = termsem τ σ i t)
-    ⇒ termsem τ σ i (s === t) = mst``,
-  rw[equation_def] >>
-  simp[termsem_def,termsem_Equal] >>
-*)
+    metis_tac[termsem_typesem,boolean_in_boolset] ) >>
+  unabbrev_all_tac >> simp[])
 
 val _ = export_theory()
